src/Language/PlutusIR/Analysis/FreeVars.v
@@ -11,7 +11,9 @@ Set Implicit Arguments.
 From PlutusCert Require Import
   Language.PlutusIR
   Language.PlutusIR.Folds
-  Util.
+  Analysis.BoundVars
+  Util
+.
 
 
 (* Parametrized for _named_ binders (not de Bruijn) *)
@@ -24,23 +26,9 @@ Section FreeVars.
 Notation term'    := (term var tyvar var tyvar).
 Notation binding' := (binding var tyvar var tyvar).
 
-Fixpoint bound_vars_binding (b : binding') : list var := match b with
-  | TermBind _ (VarDecl v _) _ => [v]
-  | DatatypeBind (Datatype _ _ matchf constructors ) => [matchf] ++ map constructorName constructors
-  | _                          => []
-  end.
 
-Fixpoint bound_vars_bindings (bs : list binding') : list var := match bs with
-    | (b :: bs)
-        => bound_vars_binding b ++ bound_vars_bindings bs
-    | nil       => nil
-    end.
 
-Fixpoint boundTerms_bindings (bs : list binding') : list (var * term var tyvar var tyvar) := match bs with
-    | ((TermBind _ (VarDecl v _) t) :: bs) => (v, t) :: boundTerms_bindings bs
-    | (b                :: bs) =>           boundTerms_bindings bs
-    | nil               => nil
-    end.
+Section fvbs.
 
 Definition delete_all : var -> list var -> list var :=
   fun x xs => filter (fun y => negb (var_eqb x y)) xs.
@@ -55,9 +43,6 @@ Definition elem x xs := existsb (var_eqb x) xs.
 
 Definition delete_all_many : list var -> list var -> list var :=
   fun ds xs => filter (fun x => negb (elem x ds)) xs.
-
-
-Section fvbs.
 (*
   Workaround for: Cannot guess decreasing argument of fix (in free_vars/free_vars_binding)
 *)
@@ -103,138 +88,4 @@ with free_vars_binding rec (b : binding') : list var :=
   .
 
 End FreeVars.
-
-
-(*
-Equations fv' : Term -> list string := {
-  fv' (Let rec bs t)    := let fvs := app (fv_bindings bs) (fv' t)
-                           in  remove_list string_dec (bound_vars_bindings bs) fvs;
-  fv' (LamAbs n ty t)   := remove string_dec n (fv' t);
-  fv' (Var n)           := n :: nil;
-  fv' (TyAbs n k t)     := fv' t;
-  fv' (Apply s t)       := fv' s ++ fv' t;
-  fv' (TyInst t ty)     := fv' t;
-  fv' (IWrap ty1 ty2 t) := fv' t;
-  fv' (Unwrap t)        := fv' t;
-  fv' (Error ty)        := nil;
-  fv' (Constant v)      := nil;
-  fv' (Builtin f)       := nil
-  }
-  where fv_bindings : list Binding -> list string := {
-    fv_bindings ((TermBind _ (VarDecl n _) t) :: bs) := cons n (fv_bindings bs) ++ fv' t;
-    fv_bindings (_                :: bs) := fv_bindings bs;
-    fv_bindings nil                      := nil
-  }
-  .
-*)
-
-(* Apparently, Equations did something special, since the similar definition below
-  is not allowed in plain gallina.
-
-  Recursive definition of fvs_bindings is ill-formed.
-  ...
-  Recursive call [in fvs_bindings] to fvs has principal argument equal to t *)
-(*
-Fixpoint fvs (t : Term) : list string := match t with
-  | (Let rec bs t)    => let vars := app (fvs_bindings bs) (fvs t)
-                         in  fold_right (remove string_dec) vars (binders bs)
-  | (Var n)           => n :: nil
-  | (TyAbs n k t)     => fvs t
-  | (LamAbs n ty t)   => remove string_dec n (fvs t)
-  | (Apply s t)       => app (fvs s) (fvs t)
-  | (TyInst t ty)     => fvs t
-  | (IWrap ty1 ty2 t) => fvs t
-  | (Unwrap t)        => fvs t
-  | (Error ty)        => nil
-  | (Constant v)      => nil
-  | (Builtin f)       => nil
-  end
-  with fvs_bindings (bs : list Binding) : list string := match bs with
-    | ((TermBind _ (VarDecl n _ ) t) :: bs) => cons n (fvs_bindings bs) ++ fvs t
-    | (b :: bs)                             => fvs_bindings bs
-    | nil                                   => nil
-    end
-.
-*)
-
-(*
-Fixpoint catMaybes {a : Type} (xs : list (option a)) : list a := match xs with
-  | nil => nil
-  | cons (Datatypes.Some x) xs => cons x (catMaybes xs)
-  | cons _ xs => catMaybes xs
-  end.
-
-Definition boundName : Binding -> option name := fun b =>
-  match b with
-    | TermBind _ (VarDecl v _) _ => Datatypes.Some v
-    | _ => None
-    end.
-
-*)
-(*
-(* TODO: use well-founded recursion to include the subterms of
-let-bindings *)
-Fixpoint free_vars (t : Term) : list name := match t with
-    | Let _ bs t   =>
-        let ts_let    := map (fun x => match x with
-          | TermBind _ _ t => Datatypes.Some t
-          | _              => None end) bs in
-        let fvs_let   := nil in (* free_vars_binders bs in *) (* TODO *)
-        let fvs_t     := free_vars t in
-        let names_let := catMaybes (map boundName bs) in
-          fold_right (remove name_dec) (app fvs_let fvs_t) names_let
-
-    | LamAbs n _ t => remove name_dec n (free_vars t)
-
-    | Var n        => n :: nil
-    | TyAbs _ _ t  => free_vars t
-    | Apply t1 t2  => free_vars t1 ++ free_vars t2
-    | TyInst t _   => free_vars t
-    | Unwrap t     => free_vars t
-    | IWrap _ _ t  => free_vars t
-    | Constant _   => nil
-    | Builtin _    => nil
-    | Error _      => nil
-    end
-.
-
-Fixpoint free_vars_binders (b : list Binding) : list name := match b with
-  | cons (TermBind _ _ t) xs => free_vars t ++ free_vars_binders xs
-  | cons _ xs => free_vars_binders xs
-  | nil => nil
-end
-.
-*)
-
-(*
-Definition fv_alg :=
-  {| A_Var      := fun n        => cons n nil
-  ;  A_LamAbs   := fun n _ fvs  => remove string_dec n fvs
-
-  ;  A_Let      := fun _ bs fvs => fvs (*TODO let bindings*)
-
-  ;  A_Apply    := fun fvs fvs' => app fvs fvs'
-  ;  A_TyAbs    := fun _ _ fvs  => fvs
-  ;  A_TyInst   := fun fvs _    => fvs
-  ;  A_IWrap    := fun _ _ fvs  => fvs
-  ;  A_Unwrap   := fun fvs      => fvs
-  ;  A_Constant := fun _        => nil
-  ;  A_Builtin  := fun _        => nil
-  ;  A_Error    := fun _        => nil
-  |}.
-
-Definition FV : Term -> list string -> Type := Fold (fv_alg).
-
-Example FV_test : FV (Var "test") (cons "test" nil).
-Proof.
-  constructor.
-Qed.
-
-Definition fv := fold (fv_alg).
-Example fv_test : fv (Var "test") = (cons "test" nil).
-Proof.
-  constructor.
-Qed.
-
-*)
 
