src/Language/PlutusIR/Transform/SplitRec.v
@@ -1,0 +1,107 @@
+From PlutusCert Require Import
+  PlutusIR
+  Analysis.FreeVars
+  Analysis.Equality
+  Analysis.UniqueBinders
+  Transform.Congruence
+  Static.Typing
+  .
+Import NamedTerm.
+Import Term.
+
+From Coq Require Import
+  Lists.List
+  Lists.ListSet
+  Strings.String
+  .
+Import ListNotations.
+
+(* A binding group (Let without a body) *)
+Definition binding_group := (Recursivity * list Binding)%type.
+
+(*
+Assuming globally unique variables, the new binding groups much satisfy:
+  - Well-scoped: each free variable in a binding RHS is bound
+  - All bindings equals those in the let-rec before transformaton
+*)
+
+Definition list_eq_elems {A} xs ys : Prop :=
+  forall (x : A), In x xs <-> In x ys.
+
+Inductive collect_binding_groups : Term -> list binding_group -> Term -> Prop :=
+  | cv_Let : forall t_body lets t_inner r bs,
+      collect_binding_groups t_body lets t_inner ->
+      collect_binding_groups (Let r bs t_body) ((r, bs) :: lets) t_inner
+  | cv_Other : forall t_inner,
+      collect_binding_groups t_inner [] t_inner
+  .
+
+Reserved Notation "t₁ ▷-split_syn t₂" (at level 30).
+Inductive split_syn : Term -> Term -> Prop :=
+  | split_rec_let : forall bs t_body t bgs t_inner,
+
+      collect_binding_groups t bgs t_inner ->
+      list_eq_elems bs (List.concat (map snd bgs)) ->
+      (*------------------------------------*)
+      (Let Rec bs t_body) ▷-split_syn t
+
+  | split_rec_cong : forall t t',
+      Cong split_syn t t' ->
+      (*--------------------*)
+      t ▷-split_syn t'
+where
+  "t1 ▷-split_syn t2" := (split_syn t1 t2)
+.
+
+
+Definition split_rec t t' :=
+  t ▷-split_syn t' /\
+  exists ty, (empty ,, empty |-+ t' : ty) /\
+  unique t'.
+
+
+Definition collect_binding_groups_dec
+     : Term -> list binding_group * Term.
+Admitted.
+
+(* Note, the below is unnecessary and implied by has_type *)
+(*
+Definition well_scoped (Γ : list string) (bg : binding_group) : Prop :=
+  match bg with
+    | (rec, bs) => forall b, In b bs ->
+        exists s v t, b = TermBind s v t /\
+          match rec with
+
+            | Rec    =>
+                incl (set_diff string_dec (free_vars String.eqb t) Γ)
+                     (free_vars_bindings String.eqb (free_vars_binding String.eqb) Rec bs)
+
+            | NonRec =>
+                exists bs_pre bs_post, bs = bs_pre ++ b :: bs_post /\
+                incl (free_vars_binding String.eqb NonRec b)
+                     (Γ ++ bound_vars_bindings bs_pre)
+          end
+  end.
+
+Fixpoint well_scoped_groups (Γ : list string) (bgs : list binding_group) : Prop :=
+  match bgs with
+    | []          => True
+    | (bg :: bgs) => well_scoped Γ bg /\ well_scoped_groups (bound_vars_bindings (snd bg) ++ Γ) bgs
+  end.
+
+Definition same_bindings (bs : list Binding) (groups : list binding_group) : Prop :=
+  let bs' := concat (map snd groups) in
+  NoDup bs ->
+  NoDup bs' ->
+  list_same_elems bs bs'.
+
+
+
+Inductive split_rec_let : list string -> binding_group -> list binding_group -> Prop :=
+  | srl : forall Γ bs groups,
+    
+    same_bindings bs groups ->
+    split_rec_let bs groups
+
+*)
+
